---
layout: post
title: "lim g(f(x)) = g(lim f(x))"
author: "Karthik"
categories: journal
tags: [documentation,sample]
---

${ \color{goldenrod}{\text{Th}} }$: Consider ${ S \overset{f}{\to} T \overset{g}{\to} \mathbb{R} }$ with ${ S,T \subseteq \mathbb{R} }.$ Say $a$ is a limit point of $S$ and ${ \lim _{x \to a } f(x) }$ exists. Also suppose ${ \lim _{x \to a} f(x) \in T }$ and $g$ is continuous at $\lim _{x \to a} f(x).$   
Then ${ \lim _{x \to a} g(f(x)) = g( \lim _{x \to a} f(x) ) }.$   
${ \color{goldenrod}{\text{Pf}} }$: Set ${ \lim _{x \to a} f(x) = \ell }.$ Let ${ \epsilon \gt 0 }.$   
There is a ${ \delta _1 \gt 0 }$ such that points ${ y \in T, \vert y - \ell \vert \lt \delta _1 }$ satisfy ${ \vert g(y) - g(\ell) \vert \lt \epsilon. }$   
There is a ${\delta _2 \gt 0 }$ such that points ${ x \in S \setminus \lbrace a \rbrace, \vert x - a \vert \lt \delta _2 }$ satisfy ${ \vert f(x) - \ell \vert \lt \delta _1.}$   
Now points ${ x \in S \setminus \lbrace a \rbrace, \vert x - a \vert \lt \delta _2 }$ satisfy ${ \vert g(f(x)) - g(\ell) \vert \lt \epsilon }.$   
So ${ \lim _{x \to a} g(f(x)) = g(\ell) },$ as needed. 

