---
layout: post
title: "Inverse of x^x (asymptotics)"
author: "Karthik"
categories: journal
tags: [documentation,sample]
---

Consider function $ f(x) = x^x $ on $ (0, \infty) $.   
$ \ln(f) = x \ln(x) $, so $ \frac{f'(x)}{f(x)} = \ln(x) + 1 $, i.e. $ f'(x) = x^x (\ln(x) + 1) $. So $ f $ is strictly increasing on ${ (\frac{1}{e}, \infty) }.$ Also ${ \lim _{x \to \infty} f(x) = \infty }.$   
So $ f : (\frac{1}{e}, \infty) \to (e^{-\frac{1}{e}}, \infty) $ is a continuous strictly increasing bijection, and therefore has a continuous strictly increasing inverse $ g $.

We'll study how $ g(y) $ behaves as $ y \to \infty $.   
Firstly $ g(y) \to \infty $ as $ y \to \infty $ : Let $ L &gt; 1 $ be given. Using $ g(y) &gt; L \iff f(g(y)) \text{ } (= y) &gt; f(L) $, we see $ g(y) &gt; L $ whenever $ y &gt; f(L) $.   


$ g(y)^{g(y)} = y $, so $g(y) \ln(g(y))  = \ln(y) $. Taking one more log, $ \ln g + \ln \ln g = \ln \ln y $, so $ 1 + \frac{\ln \ln g }{\ln g} = \frac{\ln \ln y}{\ln g} $. So as $ y \to \infty $, we see $ \frac{\ln \ln y}{\ln g} \to 1 $ (i.e. $ \ln g(y) \sim \ln \ln y $).   
Hence in the original equation $ g \ln g = \ln y $, writing $ \ln g(y) = (\ln \ln y) \psi(y) $ with $ \lim_{y \to \infty} \psi(y) = 1 $, we see $ \dfrac{g(y)}{\frac{\ln y}{\ln \ln y}} \to 1 $ as $ y \to \infty $, that is $ g(y) \sim \dfrac{\ln y}{\ln \ln y} $.  
 
